lib/smack/sesl/executor/BlockExecutor.cpp
@@ -1,4 +1,4 @@
-// Author: Xie Li
+// Author: Xie Li, Yutian Zhu
 // Institute: ISCAS
 // 2021/8/18
 #include "smack/sesl/executor/BlockExecutor.h"
